\documentclass[12pt]{article}


\usepackage{amssymb}
\usepackage{amsmath}
\usepackage{fullpage}
\usepackage{epsfig}
\usepackage{epstopdf}
\everymath{\displaystyle}



\begin{document}

\begin{center}
\underline{\LARGE{Integration by Substitution}}
\end{center}

\noindent SUGGESTED REFERENCE MATERIAL:

\medskip

\noindent As you work through the problems listed below, you should reference Chapter 5.3 of the recommended textbook (or the equivalent chapter in your alternative textbook/online resource) and your lecture notes.

\medskip

\noindent EXPECTED SKILLS:

\begin{itemize}

\item Know how to simplify a ``complicated integral" to a known form by making an appropriate substitution of variables.

\end{itemize}

\noindent PRACTICE PROBLEMS:

\medskip

\noindent {\bf For problems 1-21, evaluate the given indefinite integral and verify that your answer is correct by differentiation.}

\begin{enumerate}

\item $\int 3x^2(x^3+3)^3 \,dx$ 

\includegraphics[scale=0.5]{start.pdf}
{{$\frac{1}{4}(x^3+3)^4+C$}}
\includegraphics[scale=0.5]{end.pdf}


\item $\int \frac{5}{5x+3} \,dx$ 

\includegraphics[scale=0.5]{start.pdf}
{{$\ln{|5x+3|}+C$}}
\includegraphics[scale=0.5]{end.pdf}


\item $\int 2x\cos{(x^2)} \,dx$ 

\includegraphics[scale=0.5]{start.pdf}
{{$\sin{(x^2)}+C$}}
\includegraphics[scale=0.5]{end.pdf}


\item $\int 4x(x^2+6)^2 \,dx$ 

\includegraphics[scale=0.5]{start.pdf}
{{$\frac{2}{3}(x^2+6)^3+C$}}
\includegraphics[scale=0.5]{end.pdf}


\item $\int \sec{(4x)}\tan{(4x)} \,dx$ 

\includegraphics[scale=0.5]{start.pdf}
{{$\frac{1}{4}\sec{(4x)}+C$}}
\includegraphics[scale=0.5]{end.pdf}


\item $\int (3x-5)^{9} \,dx$ 

\includegraphics[scale=0.5]{start.pdf}
{{$\frac{1}{30}(3x-5)^{10}+C$}}
\includegraphics[scale=0.5]{end.pdf}


\item $\int e^{-2x} \,dx$ 

\includegraphics[scale=0.5]{start.pdf}
{{$-\frac{1}{2}e^{-2x}+C$}}
\includegraphics[scale=0.5]{end.pdf}


\item $\int \frac{\sin{x}\cos{x}}{1+\sin^{2}{x}} \,dx$ 

\includegraphics[scale=0.5]{start.pdf}
{{$\frac{1}{2}\ln{(1+\sin^2{x}})+C$}}
\includegraphics[scale=0.5]{end.pdf}


\item $\int \csc{\left(\frac{x}{2}\right)}\cot{\left(\frac{x}{2}\right)} \,dx$ 

\includegraphics[scale=0.5]{start.pdf}
{{$-2\csc{\left(\frac{x}{2}\right)}+C$}}
\includegraphics[scale=0.5]{end.pdf}


\item $\int -3x^3\sqrt{1-x^4} \,dx$ 

\includegraphics[scale=0.5]{start.pdf}
{{$\frac{1}{2}(1-x^{4})^{\frac{3}{2}}+C$}}
\includegraphics[scale=0.5]{end.pdf}


\item $\int \left(\frac{e^{\sqrt{x}}}{\sqrt{x}}-\frac{1}{4}\cos{4x}\right) \,dx$ 

\includegraphics[scale=0.5]{start.pdf}
{{$2e^{\sqrt{x}}-\frac{1}{16}\sin{(4x)}+C$}}
\includegraphics[scale=0.5]{end.pdf}


\item $\int \frac{1}{2+4x^2} \,dx$ 

\includegraphics[scale=0.5]{start.pdf}
{{$\frac{1}{2\sqrt{2}}\arctan{(\sqrt{2}x)}+C$}}
\includegraphics[scale=0.5]{end.pdf}


\item $\int \frac{4x}{(3+x^2)^2} \,dx$ 

\includegraphics[scale=0.5]{start.pdf}
{{$-2(3+x^2)^{-1}+C$}}
\includegraphics[scale=0.5]{end.pdf}


\item $\int x^2\sqrt{4-x} \,dx$. 

\includegraphics[scale=0.5]{start.pdf}
{{$-\frac{32}{3}(4-x)^{3/2}+\frac{16}{5}(4-x)^{5/2}-\frac{2}{7}(4-x)^{7/2}+C$}}
\includegraphics[scale=0.5]{end.pdf}


\item $\int \frac{1}{\sqrt{\frac{3}{4}+x-x^2}} \,dx$ (HINT: Complete the square)

\includegraphics[scale=0.5]{start.pdf}
{{$\arcsin{\left(x-\frac{1}{2}\right)}+C$}}
\includegraphics[scale=0.5]{end.pdf}


\item $\int{\frac{e^{3/x}}{x^2}} \,dx$

\includegraphics[scale=0.5]{start.pdf}
{{$-\frac{1}{3}e^{3/x}+C$}}
\includegraphics[scale=0.5]{end.pdf}


\item $\int \frac{e^x}{e^{2x}+1}dx$ 

\includegraphics[scale=0.5]{start.pdf}
{{$\tan^{-1}{(e^x)}+C$}}
\includegraphics[scale=0.5]{end.pdf}


\item $\int (\sin{4x})(\cos{4x})^{2/3}dx$ 

\includegraphics[scale=0.5]{start.pdf}
{{$-\frac{3}{20}(\cos{4x})^{5/3}+C$}}
\includegraphics[scale=0.5]{end.pdf}


\item $\int \csc^{2}{(3x)}\tan^{2}{(3x)}+x^2e^{x^3}dx$ 

\includegraphics[scale=0.5]{start.pdf}
{{$\frac{1}{3}\tan{(3x)}+\frac{1}{3}e^{x^3}+C$}}
\includegraphics[scale=0.5]{end.pdf}


\item $\int \frac{1}{x\ln{x}} \,dx$

\includegraphics[scale=0.5]{start.pdf}
{{$\ln{|\ln{x}|}+C$}}
\includegraphics[scale=0.5]{end.pdf}


\item $\int{\frac{\cos^{-1}{x}}{\sqrt{1-x^2}}} \,dx$

\includegraphics[scale=0.5]{start.pdf}
{{$-\frac{1}{2}\left(\cos^{-1}{x}\right)^2+C$}}
\includegraphics[scale=0.5]{end.pdf}


\item Use an appropriate trigonometric identity followed by a reasonable substitution to evaluate $\int \tan{x} \,dx$

\includegraphics[scale=0.5]{start.pdf}
{{$\ln{|\sec{x}|}+C$}}
\includegraphics[scale=0.5]{end.pdf}


\item It can be shown that $\frac{32x^2+77x+49}{(3x+1)(4x+5)^2}=\frac{2}{3x+1}-\frac{1}{(4x+5)^2}$.  Use this fact to evaluate $\int{\frac{32x^2+77x+49}{(3x+1)(4x+5)^2}} \,dx$.

\includegraphics[scale=0.5]{start.pdf}
{{$\frac{2}{3}\ln{|3x+1|}+\frac{1}{4(4x+5)}+C$}}
\includegraphics[scale=0.5]{end.pdf}


\item Using the substitution $x=\sin{\theta}$ for $-\frac{\pi}{2} \leq \theta \leq \frac{\pi}{2}$, evaluate $\int{\sqrt{1-x^2}} \,dx$.  Express your answer completely in terms of the variable $x$.\\

HINT - The following trigonometric identities will be helpful:
$\sin^2{\theta}+\cos^2{\theta}=1$, $\cos^{2}{\theta}=\frac{1}{2}(1+\cos{(2\theta})$, and $\sin{(2\theta)}=2\sin{\theta}\cos{\theta}$\\

\includegraphics[scale=0.5]{start.pdf}
{{$\frac{1}{2}x\sqrt{1-x^2}+\frac{1}{2}\sin^{-1}{x}+C$}}
\includegraphics[scale=0.5]{end.pdf}


\end{enumerate}

\end{document}