\documentclass[12pt]{article}


\usepackage{amssymb}
\usepackage{amsmath}
\usepackage{fullpage}
\usepackage{epsfig}
\usepackage{epstopdf}
\everymath{\displaystyle}



\begin{document}

\begin{center}
\underline{\LARGE{Chapter 3.2 Practice Problems}}
\end{center}

\noindent EXPECTED SKILLS:

\begin{itemize}

\item Be able to compute the derivatives of logarithmic functions.

\item Know how to use logarithmic differentiation to help find the derivatives of functions involving products and quotients.

\end{itemize}

\noindent PRACTICE PROBLEMS:

\bigskip

\noindent {\bf For problems 1-16, calculate $\frac{dy}{dx}$.}

\begin{enumerate}

\item $y = \ln{(x^2)}$ 

\includegraphics[scale=0.5]{start.pdf}
{{$\frac{2}{x}$}}
\includegraphics[scale=0.5]{end.pdf}


\item $y = \frac{1}{\ln{(3x)}}$ 

\includegraphics[scale=0.5]{start.pdf}
{{$-\frac{1}{x[\ln{(3x)}]^2}$}}
\includegraphics[scale=0.5]{end.pdf}


\item $y = x^2\ln{x}$ 

\includegraphics[scale=0.5]{start.pdf}
{{$x+2x\ln{x}$}}
\includegraphics[scale=0.5]{end.pdf}


\item $y = \ln{\left(\frac{1}{x}\right)}$ 

\includegraphics[scale=0.5]{start.pdf}
{{$-\frac{1}{x}$}}
\includegraphics[scale=0.5]{end.pdf}


\item $y = \ln|x^3|$ 

\includegraphics[scale=0.5]{start.pdf}
{{$\frac{3}{x}$}}
\includegraphics[scale=0.5]{end.pdf}


\item $y = \ln{(x^2+1)^2}$ 

\includegraphics[scale=0.5]{start.pdf}
{{$\frac{4x}{x^2+1}$}}
\includegraphics[scale=0.5]{end.pdf}


\item $y = \left[\ln{(x^2+1)}\right]^2$ 

\includegraphics[scale=0.5]{start.pdf}
{{$\frac{4x\ln{(x^2+1)}}{x^2+1}$}}
\includegraphics[scale=0.5]{end.pdf}


\item $y = \sqrt{\ln{2x}}$ 

\includegraphics[scale=0.5]{start.pdf}
{{$\frac{1}{2x\sqrt{\ln{(2x)}}}$}}
\includegraphics[scale=0.5]{end.pdf}


\item $y = \log_{2}{(3x-1)}$ 

\includegraphics[scale=0.5]{start.pdf}
{{$\frac{3}{(3x-1)\ln2}$}}
\includegraphics[scale=0.5]{end.pdf}


\item $y = \tan{(\ln{x})}$ 

\includegraphics[scale=0.5]{start.pdf}
{{$\frac{1}{x}\sec^{2}(\ln{x})$}}
\includegraphics[scale=0.5]{end.pdf}


\item $y = \ln{(\ln x)}$ 

\includegraphics[scale=0.5]{start.pdf}
{{$\frac{1}{x\ln{x}}$}}
\includegraphics[scale=0.5]{end.pdf}


\item $y=\frac{\log{x}}{2-\log{x}}$

\includegraphics[scale=0.5]{start.pdf}
{{$\frac{2}{x\ln{(10)}(2-\log{x})^2}$}}
\includegraphics[scale=0.5]{end.pdf}


\item $y=\ln{|\sec{x}|}$

\includegraphics[scale=0.5]{start.pdf}
{{$\tan{x}$}}
\includegraphics[scale=0.5]{end.pdf}


\item $y=\ln{|\sec{x}+\tan{x}|}$

\includegraphics[scale=0.5]{start.pdf}
{{$\sec{x}$}}
\includegraphics[scale=0.5]{end.pdf}


\item $y=\ln{\left(x^x\right)}$

\includegraphics[scale=0.5]{start.pdf}
{{$1+\ln(x)$}}
\includegraphics[scale=0.5]{end.pdf}


\item $y=\ln{\left(\frac{2x+1}{\sqrt{x}(3x-4)^{10}}\right)}$

\includegraphics[scale=0.5]{start.pdf}
{{$\frac{2}{2x+1}-\frac{1}{2x}-\frac{30}{3x-4}$}}
\includegraphics[scale=0.5]{end.pdf}


\item Use logarithmic differentiation to calculate $\frac{dy}{dx}$ if $y=\frac{2x+1}{\sqrt{x}(3x-4)^{10}}$

\includegraphics[scale=0.5]{start.pdf}
{{$\frac{2x+1}{\sqrt{x}(3x-4)^{10}}\left(\frac{2}{2x+1}-\frac{1}{2x}-\frac{30}{3x-4}\right)$}}
\includegraphics[scale=0.5]{end.pdf}


\item Recall the change of base formula: $\log_{b}{x}=\frac{\ln{x}}{\ln{b}}$

\begin{enumerate}

\item Remind yourself of why this is true.

\includegraphics[scale=0.5]{start.pdf}
{{{1\linewidth}{Proof:  Suppose $y=\log_b{x}$.  This is equivalent to the exponential equation $b^y=x$.  Now, we take the natural log of both sides, which gives us $\ln{(b^y)}=\ln{x}$.\\
Using a property of logarithms, we see that this is equivalent to $y\ln{b}=\ln{x}$.  Finally, we solve for $y$ by dividing both sides of the equation by $\ln{b}$, a non-zero constant since $b>0$ and $b\neq 1$.\\
Thus, $y=\frac{\ln{x}}{\ln{b}}$.}}}
\includegraphics[scale=0.5]{end.pdf}


\item Compute $y^{\prime}$ if  $y=\log_{x^2}{(e)}$

\includegraphics[scale=0.5]{start.pdf}
{{$-\frac{1}{2x(\ln{x})^2}$}}
\includegraphics[scale=0.5]{end.pdf}


\item Compute $\frac{dy}{dx}$ if $y = \log_{3x}{(x)}$ 

\includegraphics[scale=0.5]{start.pdf}
{{$\frac{\ln{3}}{x(\ln{3x})^2}$}}
\includegraphics[scale=0.5]{end.pdf}


\end{enumerate}

\item Compute an equation of the line which is tangent to the graph of $f(x)=\ln{(x^2-3)}$ at the point where $x=2$.

\includegraphics[scale=0.5]{start.pdf}
{{$y=4x-8$}}
\includegraphics[scale=0.5]{end.pdf}


\item Find the value(s) of $x$ at which the tangent line to the graph of $y=\ln{(x^2+11)}$  is perpendicular to $y=-6x+5$.

\includegraphics[scale=0.5]{start.pdf}
{{$x=1$ and $x=11$}}
\includegraphics[scale=0.5]{end.pdf}


\item Find the value(s) of $x$ at which the tangent line to the graph of $y=-\ln{x}$ passes through the origin.

\includegraphics[scale=0.5]{start.pdf}
{{$x=e$}}
\includegraphics[scale=0.5]{end.pdf}


\item Calculate $\frac{d^2y}{dx^2}$ if $y=\ln{(3x^2+2)}$.

\includegraphics[scale=0.5]{start.pdf}
{{$\frac{12-18x^2}{(3x^2+2)^2}$}}
\includegraphics[scale=0.5]{end.pdf}


\newpage

\item {\bf Multiple Choice:} Let $y=\ln{(\cos{x})}$.  Which of the following is $\frac{dy}{dx}$?

\begin{enumerate}

\item $(\ln{x})(-\sin{x})+(\cos{x})(\ln{x})$

\item $-\tan{x}$

\item $\cot{x}$

\item $\sec{x}$

\item $\frac{1}{\ln{(\cos{x})}}$

\end{enumerate}

\includegraphics[scale=0.5]{start.pdf}
{{B}}
\includegraphics[scale=0.5]{end.pdf}


\item {\bf Multiple Choice:} Let $h(x)=\ln[(f(x))^2+1]$.  Suppose that $f(1)=-1$ and $f^{\prime}(1)=1$.  Find $h^{\prime}(1)$.

\begin{enumerate}

\item $-2$

\item $-1$

\item $0$

\item $1$

\item $2$

\end{enumerate}

\includegraphics[scale=0.5]{start.pdf}
{{B}}
\includegraphics[scale=0.5]{end.pdf}


\item Consider the triangle formed by the tangent line to the graph of $y=-\ln{x}$ at the point $P(t,-\ln{t})$, the horizontal line which passes through $P$, and the $y$-axis. Find a function $A(t)$ which gives the area of this triangle.  

\includegraphics[scale=0.5]{start.pdf}
{{$A(t)=\frac{1}{2}t$}}
\includegraphics[scale=0.5]{end.pdf}


\end{enumerate}

\end{document}